SPHINCSPLUS.ec
@@ -1,0 +1,170 @@
+(* - Require/Import - *)
+(* -- Built-In (Standard Library) -- *)
+require import AllCore List Distr RealExp StdOrder.
+(*---*) import IntOrder.
+
+
+(* -- Local -- *)
+require import BinaryTrees MerkleTrees.
+require (*--*) KeyedHashFunctions TweakableHashFunctions HashAddresses.
+require (*--*) DigitalSignatures.
+require (*--*) FORS_TW FL_XMSS_MT_TW.
+
+
+
+(* - Parameters - *)
+(* 
+  Length (in bytes) of messages as well as the length of elements of 
+  private keys, public keys, and signatures
+*)
+const n : { int | 1 <= n } as ge1_n.
+
+(* Base 2 logarithm of the Winternitz parameter w *)
+const log2_w : { int | log2_w = 2 \/ log2_w = 4 \/ log2_w = 8 } as val_log2w.
+
+(* Winternitz parameter (base/radix) *)
+const w = 2 ^ log2_w. 
+
+(* Length of the message in base/radix w *)
+const len1 : int = ceil ((8 * n)%r / log2 w%r).
+
+(* Length of the checksum in base/radix w *)      
+const len2 : int = floor (log2 ((len1 * (w - 1))%r) / log2 w%r) + 1.
+
+(* Number of elements (of length n) in private keys, public keys, and signatures *)
+const len : int = len1 + len2.
+
+(* Height of a single inner tree *)
+const h' : { int | 1 <= h' } as ge1_hp. 
+
+(* Number of WOTS-TW instances of a single inner tree (i.e., number of leaves) *)
+const l' = 2 ^ h'.
+
+(* Number of layers in the hypertree (i.e., height of tree of XMSS trees) *)
+const d : { int | 1 <= d } as ge1_d.
+
+(* 
+  Height of "flattened" hypertree 
+  (i.e., total height of concatenation of inner trees) 
+*)
+const h : int = h' * d.
+
+(* 
+  Number of leaves of "flattened" hypertree
+  (i.e., total number of leaves of all inner trees on bottom layer)
+*)
+const l : int = 2 ^ h.
+ 
+(* Address type for chaining (used in tweakable hash function calls of WOTS-TW chains) *)
+const chtype : int.
+
+(* 
+  Address type for public (WOTS-TW) key compression 
+  (used in tweakable hash function calls of WOTS-TW public key compression) 
+*)
+const pkcotype : int.
+
+(* 
+  Address type for tree hashing in the hypertree 
+  (used in tweakable hash function calls of inner trees) 
+*)
+const trhmtype : int.
+
+(* 
+  Address type for tree hashing in FORS-TW trees
+  (used in tweakable hash function calls of FORS-TW trees)
+*)
+const trhftype : int.
+
+(* 
+  Address type for (FORS-TW) tree root compression
+  (used in tweakable hash function calls of FORS-TW tree root compression)
+*)
+const trcotype : int.
+
+
+(* -- Properties of parameters -- *)
+(* The different address types are distinct *)
+axiom dist_adrstypes : uniq [chtype; pkcotype; trhmtype; trhftype; trcotype].
+
+(* l' is greater than or equal to 2 *)
+lemma ge2_lp : 2 <= l'.
+proof. by rewrite /l' ler_eexpr; smt(ge1_hp). qed.
+
+(* h is greater than or equal to 1 *)
+lemma ge1_h : 1 <= h.
+proof. by rewrite /h mulr_ege1 1:ge1_hp ge1_d. qed.
+
+(* l is greater than or equal to 2 *)
+lemma ge2_l : 2 <= l.
+proof. by rewrite /l ler_eexpr; smt(ge1_h). qed.
+
+
+
+(* - Operators - *)
+(* -- Validity checks for (indices corresponding to) XMSS-MT-TW addresses -- *)
+(* Layer index validity check (note: regards hypertree) *)
+op valid_lidx (lidx : int) : bool = 
+  0 <= lidx < d.
+
+(* 
+  Tree index validity check
+  (Note: regards hypertree; i.e., is tidx a valid index for pointing to a tree in layer lidx) 
+*)
+op valid_tidx (lidx tidx : int) : bool = 
+  0 <= tidx < nr_trees lidx.
+
+(* Type index validity check *)
+op valid_typeidx (typeidx : int) : bool =
+  typeidx = chtype \/ typeidx = pkcotype \/ typeidx = trhtype.
+
+(* Key pair index validity check (note: regards inner tree) *)
+op valid_kpidx (kpidx : int) : bool =
+  0 <= kpidx < l'.
+
+(* Tree height index validity check (note: regards inner tree) *)
+op valid_thidx (thidx : int) : bool = 
+  0 <= thidx <= h'.
+  
+(* Tree breadth index validity check (note: regards inner tree) *)
+op valid_tbidx (thidx tbidx : int) : bool = 
+  0 <= tbidx < nr_nodes thidx.
+
+(* Chain index validity check *)
+op valid_chidx (chidx : int) : bool =
+  0 <= chidx < len.
+
+(* Hash index validity check *)
+op valid_hidx (hidx : int) : bool = 
+  0 <= hidx < w - 1.
+
+(* Chaining address indices validity check (local part) *) 
+op valid_xidxvalslpch (adidxs : int list) : bool =
+     valid_hidx (nth witness adidxs 0) 
+  /\ valid_chidx (nth witness adidxs 1)
+  /\ valid_kpidx (nth witness adidxs 2)
+  /\ nth witness adidxs 3 = chtype
+  /\ valid_tidx (nth witness adidxs 5) (nth witness adidxs 4)
+  /\ valid_lidx (nth witness adidxs 5).
+
+(* Public-key compression address indices validity check (local part) *)  
+op valid_xidxvalslppkco (adidxs : int list) : bool =
+     nth witness adidxs 0 = 0 
+  /\ nth witness adidxs 1 = 0
+  /\ valid_kpidx (nth witness adidxs 2)
+  /\ nth witness adidxs 3 = pkcotype
+  /\ valid_tidx (nth witness adidxs 5) (nth witness adidxs 4)
+  /\ valid_lidx (nth witness adidxs 5).
+
+(* Tree hashing address indices validity check (local part)*)  
+op valid_xidxvalslptrh (adidxs : int list) : bool =
+     valid_tbidx (nth witness adidxs 1) (nth witness adidxs 0)
+  /\ valid_thidx (nth witness adidxs 1)
+  /\ nth witness adidxs 2 = 0
+  /\ nth witness adidxs 3 = trhtype
+  /\ valid_tidx (nth witness adidxs 5) (nth witness adidxs 4)
+  /\ valid_lidx (nth witness adidxs 5).
+
+(* Local address indices validity check *)
+op valid_xidxvalslp (adidxs : int list) : bool =
+  valid_xidxvalslpch adidxs \/ valid_xidxvalslppkco adidxs \/ valid_xidxvalslptrh adidxs.
